unskipAllInside_LEMMA1z verifies - is this enough?

BROWNE.dfy
@@ -1,13 +1,19 @@
 include "Ownership.dfy"
 
-
+//pretty sure the main point of this entire file
+//is to prove that skipAllInside(o,pivot) == arghStrictlyInside)(o,pivot)
+//i.e,.                                   == allStrictlyInside(argh(o),pivot)
 //
+// skip all inside is recursive & terminates early;
+//  allStrictlyInside is iteraative sugar for a set comprehension.
 //
 //   assert (set x <- next.AMFO | strictlyInside(x,m.o)) == skipAllInside(next,m.o);
 //   assert (set x <- cext.AMFO | strictlyInside(x,m.c)) == skipAllInside(cext,m.c);
 
 
 function skipAllInside(o : Object, pivot : Object) : (rv : set<Object>)
+  // all o's transitive owners strictly inside pivot
+  // recursive, shortcutting analogue of allInside
   decreases o.AMFO
    requires o.Ready()
     {
@@ -16,14 +22,15 @@ function skipAllInside(o : Object, pivot : Object) : (rv : set<Object>)
     }
 
 function unskipAllInside(o : Object, pivot : Object) : (rv : set<Object>)
-  decreases o.AMFO
+  // all o's transitive owners strictly inside pivot
+  // recursive, NON-shortcutting analogue of allInside - skipAllInside
+    decreases o.AMFO
    requires o.Ready()
     {
-      if (not(strictlyInside(o,pivot))) then (set oo <- o.owner, ooo <- unskipAllInside(oo, pivot) :: ooo)
+      if (not(strictlyInside(o,pivot)))
+          then        (set oo <- o.owner, ooo <- unskipAllInside(oo, pivot) :: ooo)
           else  {o} + (set oo <- o.owner, ooo <- unskipAllInside(oo, pivot) :: ooo)
     }
-
-
 
 
 lemma {:timeLimit 3} unskipAllInside_LEMMA0(o : Object, pivot : Object, skip : Owner, unskip : Owner)
@@ -48,7 +55,7 @@ lemma {:timeLimit 3} unskipAllInside_LEMMA0(o : Object, pivot : Object, skip : O
       assert o in skip;
       assert o in unskip;
 
-assert o.Ready(); assert AllReady(o.owner);
+      assert o.Ready(); assert AllReady(o.owner);
       forall oo <- o.owner
         ensures (unskipAllInside(oo, pivot) == skipAllInside(oo, pivot)) {
             assert o.AMFO decreases to oo.AMFO;
@@ -57,17 +64,21 @@ assert o.Ready(); assert AllReady(o.owner);
             unskipAllInside_LEMMA0(oo, pivot, oo_skip, oo_unskip);
             assert oo_skip == oo_unskip;
       }
-
    }
 
 
 
 
+
+
+
 lemma unskipAllInside_LEMMA1(o : Object, pivot : Object)
+  //unskip outside pivot is always empty
   decreases o.AMFO
    requires o.Ready()
    requires (not(strictlyInside(o,pivot)))
     ensures unskipAllInside(o, pivot) == {}
+    ensures forall r <- unskipAllInside(o, pivot) :: strictlyInside(o, pivot)
    {
       forall oo <- o.owner
         ensures (unskipAllInside(o, pivot) == {})
@@ -75,39 +86,423 @@ lemma unskipAllInside_LEMMA1(o : Object, pivot : Object)
          argh_LEMMA2(oo,pivot);
          assert (not(strictlyInside(oo,pivot)));
          unskipAllInside_LEMMA1(oo,pivot);
-         assert unskipAllInside(o, pivot) == {};
+         assert unskipAllInside(oo, pivot) == {};
         }
 
    }
 
-lemma {:timeLimit 60} unskipAllInside_LEMMA2(o : Object, pivot : Object, unskip : Owner)
+
+
+lemma unskipAllInside_LEMMA1i(o : Object, pivot : Object)
+  //unskip results are always strictlyInsice
   decreases o.AMFO
    requires o.Ready()
-   requires strictlyInside(o,pivot)
-   requires unskip == unskipAllInside(o,pivot)
-//    ensures unskipAllInside(o, pivot) == {o} + (set oo <- o.owner, ooo <- unskipAllInside(oo, pivot) :: ooo)
-{
+   ensures forall r <- unskipAllInside(o, pivot) :: strictlyInside(r, pivot)
+   { }
 
-assert o in unskip;
 
-assert strictlyInside(o,pivot);
 
-forall oo <- o.owner, ooo <- unskipAllInside(oo, pivot)
-  ensures true
-    {
-      if (strictlyInside(oo,pivot))
-        {
+lemma unskipAllInside_LEMMA1a(o : Object, pivot : Object)
+  //unskip is always from tranwitive ownerhsip (AMFO/argh)
+  decreases o.AMFO
+   requires o.Ready()
+    ensures forall r <- unskipAllInside(o, pivot) :: (r in argh(o))
+    ensures unskipAllInside(o, pivot) <= argh(o)
+   { }
 
-        }
+
+
+lemma unskipAllInside_LEMMA1n(o : Object, pivot : Object)
+  //if I'm inside I should be in unskipaAllInsidestrictlyInside
+  decreases o.AMFO
+   requires o.Ready()
+    ensures forall x <- argh(o) | not(strictlyInside(x, pivot)) :: (x !in unskipAllInside(o, pivot))
+   {
+     unskipAllInside_LEMMA1i(o,pivot);
+     assert forall r <- unskipAllInside(o, pivot) :: strictlyInside(r, pivot);
+
+   }
+
+
+
+lemma unskipAllInside_LEMMA1o(o : Object, pivot : Object, x : Object)
+  //if I'm inside I should be in unskipaAllInsidestrictlyInside
+  decreases o.AMFO
+   requires o.Ready()
+   requires x in argh(o)
+   requires strictlyInside(x,pivot)
+    ensures x in unskipAllInside(o, pivot)
+   {
+      if (x == o) {assert x in unskipAllInside(o, pivot); return;}
+      assert x != o;
+
+//      if (x in o.owner) {assert x in unskipAllInside(o, pivot); return;}
+
+      assert exists oo <- o.owner, xx <- argh(oo) :: x == xx;
+      assert exists oo <- o.owner :: x in unskipAllInside(oo, pivot);
     }
 
 
 
- assert unskipAllInside(o,pivot) ==  //ERR
-       if (not(strictlyInside(o,pivot))) then (set oo <- o.owner, ooo <- unskipAllInside(oo, pivot) :: ooo)
-          else  {o} + (set oo <- o.owner, ooo <- unskipAllInside(oo, pivot) :: ooo);
+lemma unskipAllInside_LEMMA1z(o : Object, pivot : Object)
+  //if I'm inside I should be in unskipaAllInsidestrictlyInside
+  decreases o.AMFO
+   requires o.Ready()
+    ensures forall oo <- argh(o) | strictlyInside(oo,pivot) :: oo in unskipAllInside(o, pivot)
 
+    ensures (set oo <- argh(o) | strictlyInside(oo,pivot)) <= unskipAllInside(o, pivot)
+    ensures (set oo <- argh(o) | strictlyInside(oo,pivot)) >= unskipAllInside(o, pivot)
+    ensures (set oo <- argh(o) | strictlyInside(oo,pivot)) == unskipAllInside(o, pivot)
+
+    ensures (set oo <- argh(o) | strictlyInside(oo,pivot)) <= arghStrictlyInside(o, pivot)
+    ensures (set oo <- argh(o) | strictlyInside(oo,pivot)) >= arghStrictlyInside(o, pivot)
+    ensures (set oo <- argh(o) | strictlyInside(oo,pivot)) == arghStrictlyInside(o, pivot)
+
+    ensures arghStrictlyInside(o,pivot) == unskipAllInside(o, pivot)
+   {
+    forall oo <- argh(o) | strictlyInside(oo,pivot) ensures ( oo in unskipAllInside(o, pivot) )  {   //oo in unskipAllInside(o, pivot)
+       assert o.Ready();
+       assert oo in argh(o);
+       assert strictlyInside(oo,pivot);
+       unskipAllInside_LEMMA1o(o,pivot,oo);
+       assert oo in unskipAllInside(o, pivot);
+      }
+
+    }
+
+
+
+
+
+//close up
+
+
+
+
+
+
+
+
+
+
+
+
+
+
+lemma {:timeLimit 30} unskipAllInside_LEMMA2(o : Object, pivot : Object, arghIn : Owner, unskip : Owner)
+  //unskip equals arghInside4\
+  decreases o.AMFO
+   requires o.Ready()
+   requires pivot.Ready()
+   requires arghIn == arghStrictlyInside(o, pivot)
+   requires unskip == unskipAllInside(o, pivot)
+    ensures forall oo <- o.owner :: unskipAllInside(oo, pivot) == arghStrictlyInside(oo, pivot)
+
+    ensures unskip == arghIn
+   {
+      if (not(strictlyInside(o,pivot)))
+        {
+         arghStrictlyInside_LEMMA1(o,pivot);
+         assert arghStrictlyInside(o, pivot) == {};
+         unskipAllInside_LEMMA1(o,pivot);
+         assert unskipAllInside(o, pivot) == {};
+         assert unskip == arghIn;
+         return;
+        }
+
+      assert strictlyInside(o,pivot);
+
+      assert o in arghIn;
+      assert o in unskip;
+
+      assert o.Ready(); assert AllReady(o.owner);
+
+      forall oo <- o.owner
+        ensures (unskipAllInside(oo, pivot) == arghStrictlyInside(oo, pivot)) {
+            assert o.AMFO decreases to oo.AMFO;
+            var oo_arghIn := arghStrictlyInside(oo, pivot);
+            var oo_unskip := unskipAllInside(oo, pivot);
+            unskipAllInside_LEMMA2(oo, pivot, oo_arghIn, oo_unskip);
+            assert oo_arghIn == oo_unskip;
+        }
+
+      assert forall oo <- o.owner :: unskipAllInside(oo, pivot) == arghStrictlyInside(oo, pivot);
+
+      unskipAllInside_LEMMA3(o,pivot);
+
+//       assert (set oo <- o.owner, ooo <- unskipAllInside(oo, pivot) :: ooo) == (set oo <- o.owner, ooo <- arghStrictlyInside(oo, pivot) :: ooo);
+//
+//
+//       assert unskip == {o} + (set oo <- o.owner, ooo <- unskipAllInside(oo, pivot) :: ooo);
+//
+//     assert arghIn == arghStrictlyInside(o, pivot) == allStrictlyInside(argh(o),pivot) == (set x <- argh(o) | strictlyInside(x,pivot));
+// argh_LEMMA0(o); cunty_LEMMA4(o,pivot);
+//     assert arghIn == (set x <- argh(o) | strictlyInside(x,pivot))
+//                   == (set x <- ({o} + (set oo <- o.owner, ooo <- argh(oo) :: ooo))  | strictlyInside(x,pivot));
+
+
+    assert (set x <- ({o} + (set oo <- o.owner, ooo <- argh(oo) :: ooo))  | strictlyInside(x,pivot))
+        == (set x <- {o} | strictlyInside(x,pivot)) + (set x <- (set oo <- o.owner, ooo <- argh(oo) :: ooo)  | strictlyInside(x,pivot)); //ERR
+
+    assert (set x <- {o} | strictlyInside(x,pivot)) == {o}  by {  assert strictlyInside(o,pivot); } //ERR
+
+    // assert (set x <- (set oo <- o.owner, ooo <- argh(oo) :: ooo)  | strictlyInside(x,pivot))
+    //     ==           (set oo <- o.owner, ooo <- argh(oo) | strictlyInside(oo,pivot) :: ooo ) //ERR
+    //     ==           (set oo <- o.owner, ooo <- arghStrictlyInside(oo,pivot) :: ooo); //ERR
+
+
+      forall oo <- o.owner
+        ensures (unskipAllInside(oo, pivot) == arghStrictlyInside(oo, pivot)) {
+            assert o.AMFO decreases to oo.AMFO;
+            var oo_arghIn := arghStrictlyInside(oo, pivot);
+            var oo_unskip := unskipAllInside(oo, pivot);
+            unskipAllInside_LEMMA2(oo, pivot, oo_arghIn, oo_unskip);
+            assert oo_arghIn == oo_unskip;
+        }
+
+assert        (set oo <- o.owner, ooo <- arghStrictlyInside(oo,pivot) :: ooo) ==        (set oo <- o.owner, ooo <- unskipAllInside(oo, pivot) :: ooo);
+
+assert  {o} + (set oo <- o.owner, ooo <- arghStrictlyInside(oo,pivot) :: ooo) == {o} +  (set oo <- o.owner, ooo <- unskipAllInside(oo, pivot) :: ooo);
+
+// assert  arghStrictlyInside(o,pivot) == unskipAllInside(o, pivot); //ERR
+
+//
+//       // assert arghIn == {o} + (set oo <- o.owner, ooo <- arghStrictlyInside(oo, pivot) :: ooo)  //ERR
+//       //    by {  assert strictlyInside(o,pivot); }
+//
+      assert unskip == arghIn;
+
+   }
+
+
+
+lemma unskipAllInside_LEMMA3(o : Object, pivot : Object)   //WORKS
+ //given unskipAllInside owners == arghStrictlyInside owners
+ //then  set of unskips is set of arghStrictlyInside
+   decreases o.AMFO
+    requires o.Ready()
+    requires pivot.Ready()
+    requires strictlyInside(o,pivot)
+    requires forall oo <- o.owner :: unskipAllInside(oo, pivot) == arghStrictlyInside(oo, pivot)
+
+   // these two doesn't work
+   //   ensures forall oo <- o.owner :: ((set ooo <- unskipAllInside(oo, pivot) :: ooo) == (set ooo <- arghStrictlyInside(oo, pivot) :: ooo))
+   //   ensures (set oo <- o.owner, ooo <- unskipAllInside(oo, pivot) :: ooo) == (set oo <- o.owner, ooo <- arghStrictlyInside(oo, pivot) :: ooo)
+
+     ensures forall oo <- o.owner :: (set ooo <- unskipAllInside(oo,pivot) :: ooo) == (set ooo <- arghStrictlyInside(oo,pivot) :: ooo)
+     ensures (set oo <- o.owner, ooo <- (set x <- unskipAllInside(oo,pivot)) :: ooo) == (set oo <- o.owner, ooo <- arghStrictlyInside(oo,pivot) :: ooo)
+     ensures (set oo <- o.owner, ooo <- unskipAllInside(oo,pivot) :: ooo) == (set oo <- o.owner, ooo <- arghStrictlyInside(oo,pivot) :: ooo)
+
+{
+   forall oo <- o.owner ensures ((set ooo <- unskipAllInside(oo, pivot) :: ooo) == (set ooo <- arghStrictlyInside(oo, pivot) :: ooo))
+      {
+         assert unskipAllInside(oo, pivot) == arghStrictlyInside(oo, pivot);
+      }
+
+   assert forall oo <- o.owner ::  ((set ooo <- unskipAllInside(oo, pivot) :: ooo) == (set ooo <- arghStrictlyInside(oo, pivot) :: ooo));
 }
+
+lemma setequals_LEMMA0(o : Object, left : Owner, right : Owner)
+ requires left == right
+  ensures {o} + left == {o} + right
+{}
+
+
+
+lemma unskipAllInside_LEMMA4(o : Object, pivot : Object, left : Owner, rite : Owner)
+   decreases o.AMFO
+    requires o.Ready()
+    requires pivot.Ready()
+    // requires strictlyInside(o,pivot)
+    requires left == (set oo <- o.owner, ooo <- unskipAllInside(oo,pivot) :: ooo)
+    requires rite == (set oo <- o.owner, ooo <- arghStrictlyInside(oo,pivot) :: ooo)
+    requires left == rite
+     ensures {o} + left == {o} + rite
+{
+  setequals_LEMMA0(o,left,rite);
+}
+
+
+lemma cunty_LEMMA5(o : Object, pivot : Object, left : Owner)
+   decreases o.AMFO
+    requires o.Ready()
+    requires pivot.Ready()
+    requires strictlyInside(o,pivot)
+    requires left == {o} + (set oo <- o.owner, ooo <- unskipAllInside(oo,pivot) :: ooo)
+     ensures left == unskipAllInside(o,pivot)
+{
+}
+
+lemma unskipAllInside_LEMMA5(o : Object, pivot : Object, rv : Owner)
+   decreases o.AMFO
+    requires o.Ready()
+    requires pivot.Ready()
+    requires rv ==  unskipAllInside(o,pivot)
+    requires strictlyInside(o,pivot)
+     ensures o in rv
+     ensures (set oo <- o.owner, ooo <- unskipAllInside(oo, pivot) :: ooo) <= rv
+     ensures forall r <- rv :: (r == o) || (r in  (set oo <- o.owner, ooo <- unskipAllInside(oo, pivot) :: ooo) )
+    //  ensu
+//    res rv <= {o} + (set oo <- o.owner, ooo <- unskipAllInside(oo, pivot) :: ooo)
+    //  ensures rv >= {o} + (set oo <- o.owner, ooo <- unskipAllInside(oo, pivot) :: ooo)
+
+{
+  //  if (not(strictlyInside(o,pivot)))
+  //     {
+  //         assert unskipAllInside(o,pivot) == (set oo <- o.owner, ooo <- unskipAllInside(oo, pivot) :: ooo);
+  //     } else {
+  //         assert unskipAllInside(o,pivot) == {o} + (set oo <- o.owner, ooo <- unskipAllInside(oo, pivot) :: ooo);
+  //     }
+}
+
+
+
+
+
+
+
+lemma unskipAllInside_LEMMA6(o : Object, pivot : Object)
+
+   decreases o.AMFO
+    requires o.Ready()
+    requires pivot.Ready()
+//  requires strictlyInside(o,pivot)
+     ensures unskipAllInside(o,pivot)    == {o} + (set oo <- o.owner, ooo <- unskipAllInside(oo,pivot) :: ooo)
+     ensures arghStrictlyInside(o,pivot) == {o} + (set oo <- o.owner, ooo <- arghStrictlyInside(oo,pivot) :: ooo)
+{}
+
+
+
+
+
+
+
+
+lemma cunty_LEMMA3(o : Object, pivot : Object)
+ //lifts asI==sAi to sets
+   decreases o.AMFO
+    requires o.Ready()
+    requires pivot.Ready()
+    requires strictlyInside(o,pivot)
+    requires forall oo <- o.owner :: argh(oo) == oo.AMFO
+
+   // these two doesn't work
+   //   ensures forall oo <- o.owner :: ((set ooo <- unskipAllInside(oo, pivot) :: ooo) == (set ooo <- arghStrictlyInside(oo, pivot) :: ooo))
+   //   ensures (set oo <- o.owner, ooo <- unskipAllInside(oo, pivot) :: ooo) == (set oo <- o.owner, ooo <- arghStrictlyInside(oo, pivot) :: ooo)
+
+     ensures forall oo <- o.owner :: (set ooo <- argh(oo) :: ooo) == (set ooo <- oo.AMFO :: ooo)
+     ensures (set oo <- o.owner, ooo <- (set x <- argh(oo)) :: ooo) == (set oo <- o.owner, ooo <- oo.AMFO :: ooo)
+     ensures (set oo <- o.owner, ooo <- argh(oo) :: ooo) == (set oo <- o.owner, ooo <- oo.AMFO :: ooo)
+
+{
+   forall oo <- o.owner ensures ((set ooo <- argh(oo) :: ooo) == (set ooo <- oo.AMFO :: ooo))
+      {
+         assert argh(oo) == oo.AMFO;
+      }
+
+   assert forall oo <- o.owner ::  ((set ooo <- argh(oo) :: ooo) == (set ooo <- oo.AMFO :: ooo));
+}
+
+
+
+
+lemma cunty_LEMMA4(o : Object, pivot : Object)
+ //lifts asI==sAi to sets
+   decreases o.AMFO
+    requires o.Ready()
+    requires pivot.Ready()
+    requires strictlyInside(o,pivot)
+    requires forall oo <- o.owner :: argh(oo) == oo.AMFO
+
+     ensures (set oo <- o.owner, ooo <- argh(oo) :: ooo) == (set oo <- o.owner, ooo <- oo.AMFO :: ooo)
+     ensures ({o} + (set oo <- o.owner, ooo <- argh(oo) :: ooo)) == ({o} + (set oo <- o.owner, ooo <- oo.AMFO :: ooo))
+     ensures argh(o) == ({o} + (set oo <- o.owner, ooo <- argh(oo) :: ooo))
+     ensures argh(o) == ({o} + (set oo <- o.owner, ooo <- oo.AMFO :: ooo))
+
+{
+  cunty_LEMMA3(o,pivot);
+}
+
+
+lemma arghStrictlyInside_LEMMA1(o : Object, pivot : Object)
+    //arghStrictlyInside outside pivot is always empty
+  decreases o.AMFO
+   requires o.Ready()
+   requires (not(strictlyInside(o,pivot)))
+    ensures arghStrictlyInside(o, pivot) == {}
+   {
+      forall oo <- o.owner
+        ensures (arghStrictlyInside(o, pivot) == {})
+        {
+         argh_LEMMA2(oo,pivot);
+         assert (not(strictlyInside(oo,pivot)));
+         arghStrictlyInside_LEMMA1(oo,pivot);
+         assert arghStrictlyInside(o, pivot) == {};
+        }
+
+   }
+
+
+lemma  arghStrictlyInside_LEMMA5(o : Object, pivot : Object, arghIn : Owner)
+  //control flow "inversion" of arghStrictlyInside...
+  decreases o.AMFO
+   requires o.Ready()
+   requires pivot.Ready()
+   requires arghIn == arghStrictlyInside(o, pivot)
+   requires strictlyInside(o,pivot)
+   // ensures arghIn == {o} + (set oo <- o.owner, ooo <- arghStrictlyInside(oo, pivot) :: ooo)
+{
+   assert arghIn == arghStrictlyInside(o, pivot);
+   assert arghIn == allStrictlyInside(argh(o),pivot);
+   assert arghIn == (set oo <- argh(o) | strictlyInside(oo,pivot));
+   argh_LEMMA4(o);
+   assert arghIn == (set oo <- ({o} + (set oo <- o.owner, ooo <- argh(oo) :: ooo))  | strictlyInside(oo,pivot)); //ERR
+}
+
+
+
+lemma arghStrictlyInside_LEMMA6(o : Object, pivot : Object, arghIn : Owner)
+  //control flow "inversion" of arghStrictlyInside...
+  decreases o.AMFO
+   requires o.Ready()
+   requires pivot.Ready()
+   requires strictlyInside(o,pivot)
+   requires arghIn == (set oo <- argh(o) | strictlyInside(oo,pivot))
+   // ensures arghIn == {o} + (set oo <- o.owner, ooo <- arghStrictlyInside(oo, pivot) :: ooo)
+{
+   assert arghIn == (set oo <- argh(o) | strictlyInside(oo,pivot));
+   assert arghIn == (set oo <- ({o} + (set oo <- o.owner, ooo <- argh(oo) :: ooo))  | strictlyInside(oo,pivot)); //ERR
+}
+
+
+
+lemma arghStrictlyInside_LEMMA7(o : Object, pivot : Object, arghIn : Owner)
+  //control flow "inversion" of arghStrictlyInside...
+  decreases o.AMFO
+   requires o.Ready()
+   requires pivot.Ready()
+   requires strictlyInside(o,pivot)
+   requires AllReady(arghIn)
+   requires arghIn == argh(o)
+    ensures argh(o) == o.AMFO
+    ensures argh(o) == {o} + (set oo <- o.owner, ooo <- argh(oo) :: ooo)   //ERR
+   {
+         argh_LEMMA4(o);
+   }
+
+
+
+// lemma unskipAllInside_LEMMA4(o : Object, pivot : Object)   //WORKS
+//    decreases o.AMFO
+//     requires o.Ready()
+//     requires pivot.Ready()
+//     requires strictlyInside(o,pivot)
+//     requires forall oo <- o.owner ::  ((set ooo <- unskipAllInside(oo, pivot) :: ooo) == (set ooo <- arghStrictlyInside(oo, pivot) :: ooo))
+//      ensures (set oo <- o.owner, ooo <- unskipAllInside(oo, pivot) :: ooo) == (set oo <- o.owner, ooo <- arghStrictlyInside(oo, pivot) :: ooo)
+// {}
+
+
+
 
 //
 // lemma skipAllInside_LEMMA1(next : Object, pivot : Object)  //FAILS
@@ -176,13 +571,13 @@ forall oo <- o.owner, ooo <- unskipAllInside(oo, pivot)
 
 
 
-lemma skipAllInside_LEMMA1a(o : Object, pivot : Object)   ///DOESNT WORK
+lemma skipAllInside_LEMMA1a(o : Object, pivot : Object)   ///DOESNT WORK - calls UNPROVED subLEMMERS
    decreases o.AMFO
     requires o.Ready()
     requires pivot.Ready()
 //    requires strictlyInside(o,pivot)
 //     ensures forall oo <- o.owner :: allStrictlyInside(oo.AMFO,pivot) == skipAllInside(oo,pivot)
-  ensures allStrictlyInside(o.AMFO,pivot) == skipAllInside(o,pivot)
+     ensures allStrictlyInside(o.AMFO,pivot) == skipAllInside(o,pivot)
 {
       if (not(strictlyInside(o,pivot)))
         {
@@ -244,7 +639,7 @@ lemma skipAllInside_LEMMA1b(o : Object, pivot : Object)   //WORKS
       }
 }
 
-lemma skipAllInside_LEMMA1c(o : Object, pivot : Object, aSI : Owner, sAI : Owner)   //DIESBT WOIRKJ
+lemma skipAllInside_LEMMA1c(o : Object, pivot : Object, aSI : Owner, sAI : Owner)   //DOESNT WORK
    decreases o.AMFO
     requires o.Ready()
     requires pivot.Ready()
@@ -320,15 +715,15 @@ lemma arghStrictlyInside_LEMMA1b(o : Object, pivot : Object)   //WORKS
 
 
 // {:timeLimit 30}
-lemma argh_LEMMMA3(o : Object, pivot : Object)
+lemma argh_LEMMA13(o : Object, pivot : Object)  //doesn't work without assume
    decreases o.AMFO
     requires o.Ready()
     requires pivot.Ready()
-     ensures arghStrictlyInside(o,pivot) == skipAllInside(o,pivot)
+     ensures arghStrictlyInside(o,pivot) == skipAllInside(o,pivot)//ERR
 {
         if (not(strictlyInside(o,pivot)))
         {
-            argh_LEMMMA3a(o,pivot);
+            argh_LEMMA13a(o,pivot);
             assert arghStrictlyInside(o,pivot) == {};
             assert arghStrictlyInside(o,pivot) == skipAllInside(o,pivot) == {};
             return;
@@ -349,7 +744,7 @@ lemma argh_LEMMMA3(o : Object, pivot : Object)
        forall oo <- o.owner
          ensures arghStrictlyInside(oo,pivot) == skipAllInside(oo,pivot)
          {
-           argh_LEMMMA3(oo,pivot);
+           argh_LEMMA13(oo,pivot);
            assert arghStrictlyInside(oo,pivot) == skipAllInside(oo,pivot);
          }
 
@@ -362,11 +757,11 @@ assert  (set oo <- o.owner, ooo <- arghStrictlyInside(oo,pivot) :: ooo) ==
 
       assert skipAllInside(o,pivot) == {o} + (set oo <- o.owner, ooo <- skipAllInside(oo,pivot) :: ooo);
 
-assume  arghStrictlyInside(o,pivot) == skipAllInside(o,pivot);
+// assume  arghStrictlyInside(o,pivot) == skipAllInside(o,pivot);
 }
 
 
-lemma  {:timeLimit 30} argh_LEMMMA3a(o : Object, pivot : Object)
+lemma  {:timeLimit 30} argh_LEMMA13a(o : Object, pivot : Object)
    decreases o.AMFO
     requires o.Ready()
     requires pivot.Ready()
@@ -378,23 +773,19 @@ lemma  {:timeLimit 30} argh_LEMMMA3a(o : Object, pivot : Object)
 }
 
 //allStrictlyInside(argh(o),pivot)
-lemma {:timeLimit 30} argh_LEMMMA3b(o : Object, pivot : Object)  //DOES NOTHING
-   decreases o.AMFO
-    requires o.Ready()
-    requires pivot.Ready()
-    requires (strictlyInside(o,pivot))
-    requires o.owner > {}
- //    ensures arghStrictlyInside(o,pivot) == {o} + (set oo <- o.owner, ooo <- arghStrictlyInside(oo,pivot) :: ooo);
-{
-  assert arghStrictlyInside(o,pivot)  == allStrictlyInside(argh(o),pivot);
+// lemma {:timeLimit 30} argh_LEMMA13b(o : Object, pivot : Object)  //DOES NOTHING
+//    decreases o.AMFO
+//     requires o.Ready()
+//     requires pivot.Ready()
+//     requires (strictlyInside(o,pivot))
+//     requires o.owner > {}
+//  //    ensures arghStrictlyInside(o,pivot) == {o} + (set oo <- o.owner, ooo <- arghStrictlyInside(oo,pivot) :: ooo);
+// {
+//   assert arghStrictlyInside(o,pivot)  == allStrictlyInside(argh(o),pivot);
+// //  assert arghStrictlyInside(o,pivot)  == allStrictlyInside(argh(o),pivot);
+// }
 
-
-
-//  assert arghStrictlyInside(o,pivot)  == allStrictlyInside(argh(o),pivot);
-
-}
-
-lemma {:timeLimit 30} argh_LEMMMA3c(o : Object, a : Owner, pivot : Object)
+lemma {:timeLimit 30} argh_LEMMA13c(o : Object, a : Owner, pivot : Object)
    decreases o.AMFO
     requires o.Ready()
     requires a == argh(o)
@@ -409,13 +800,13 @@ lemma {:timeLimit 30} argh_LEMMMA3c(o : Object, a : Owner, pivot : Object)
      ensures allStrictlyInside(a,pivot) == (set o : Object <- a | strictlyInside(o,pivot))
      {
          argh_LEMMA3(o);
-         argh_LEMMMA3d(a,pivot);
+         argh_LEMMA13d(a,pivot);
 
          assert allStrictlyInside(a,pivot) == (set o : Object <- a | strictlyInside(o,pivot));
      }
 
 
-lemma {:timeLimit 30} argh_LEMMMA3d(oo : Owner, pivot : Object)
+lemma {:timeLimit 30} argh_LEMMA13d(oo : Owner, pivot : Object)
     requires AllReady(oo)
     requires pivot.Ready()
      ensures allStrictlyInside(oo,pivot) ==  (set o : Object <- oo | strictlyInside(o,pivot) )
@@ -424,17 +815,76 @@ lemma {:timeLimit 30} argh_LEMMMA3d(oo : Owner, pivot : Object)
 
 
 function argh(o : Object) : (rv : Owner)
-//clean recursive alter alternative definition of AMFO (recAmfo?)
+//clean recursive alter alternative definition of AMFO (recAmfo?) // recAllOwners
   decreases o.AMFO
   // requires o.Ready()
  { assume o.Ready();
    {o} + (set oo <- o.owner, ooo <- argh(oo) :: ooo) }
+
+
+// lemma argh_LEMMA00(o : Object)
+// //establishes o.AMFO == argh(o)
+//   decreases o.AMFO
+//    requires o.Ready()
+//  //   ensures argh(o) == ({o} + (set oo <- o.owner, ooo <- argh(oo) :: ooo))
+// {
+//     assert argh(o) == o.AMFO by { argh_LEMMA0(o); }
+//     assert argh(o) == ({o} + (set oo <- o.owner, ooo <- oo.AMFO :: ooo))
+//       by { argh_LEMMA4(o); assert (argh(o) == ({o} + (set oo <- o.owner, ooo <- oo.AMFO :: ooo))); }
+//     forall oo <- o.owner ensures (oo.AMFO == argh(oo)) {argh_LEMMA0(oo); }
+//
+//     assert argh(o) == ({o} + (set oo <- o.owner, ooo <- argh(oo) :: ooo));
+// }
+
+
+// lemma argh_LEMMA00(o : Object)
+// //establishes o.AMFO == argh(o)
+//   decreases o.AMFO
+//    requires o.Ready()
+//     ensures argh(o) == ({o} + (set oo <- o.owner, ooo <- argh(oo) :: ooo))
+// {
+//    if (o.owner == {}) {return;}
+//
+//    forall oo <- o.owner ensures (argh(oo) == ({oo} + (set xx <- oo.owner, xxx <- argh(xx) :: xxx)))
+//    {
+//       argh_LEMMA00(oo);
+//       assert argh(oo) == ({oo} + (set xx <- oo.owner, xxx <- argh(xx) :: xxx));
+//    }
+//
+//
+//    forall oo <- o.owner ensures (argh(oo) == ({oo} + (set xx <- oo.owner, xxx <- argh(xx) :: xxx)))
+//    {
+//       argh_LEMMA00(oo);
+//       assert argh(oo) == ({oo} + (set xx <- oo.owner, xxx <- argh(xx) :: xxx));
+//    }
+//
+// //   assert forall oo <- o.owner :: (argh(oo) == ({oo} + (set xx <- oo.owner, xxx <- argh(xx) :: xxx)));
+//
+// }
+
+
+lemma arghStrictlyInside_LEMMA0(o : Object)
+//establishes o.AMFO == argh(o)
+  decreases o.AMFO
+   requires o.Ready()
+    ensures o.AMFO == argh(o)
+{
+   if (o.owner == {}) {return;}
+
+   forall oo <- o.owner ensures (true)
+   {
+      argh_LEMMA0(oo);
+      assert argh(oo) == oo.AMFO;
+   }
+}
+
 
 lemma argh_LEMMA0(o : Object)
 //establishes o.AMFO == argh(o)
   decreases o.AMFO
    requires o.Ready()
     ensures o.AMFO == argh(o)
+    ensures forall oo <- o.owner :: argh(oo) == oo.AMFO
 {
    if (o.owner == {}) {return;}
 
@@ -462,13 +912,49 @@ lemma argh_LEMMA2(o : Object, pivot : Object)   //ONCE_OUTSIDE_ALL_OUTSIDE
 {}
 
 lemma argh_LEMMA3(o : Object)
- //deconstructs AMFO to iteration over *owners*
+ //result of argh are ready
   decreases o.AMFO
    requires o.Ready()
     ensures AllReady( argh(o) )
 {
    argh_LEMMA0(o);
 }
+
+
+lemma argh_LEMMA4(o : Object)
+ //deconstructs AMFO to iteration over *owners*
+  decreases o.AMFO
+   requires o.Ready()
+    ensures argh(o) == ({o} + (set oo <- o.owner, ooo <- oo.AMFO :: ooo))
+{
+     argh_LEMMA0(o);
+}
+
+lemma argh_LEMMA5(o : Object)
+  decreases o.AMFO
+   requires o.Ready()
+    ensures argh(o) == ({o} + (set oo <- o.owner, ooo <- argh(oo) :: ooo))//ERR
+{
+     argh_LEMMA4(o);
+     assert argh(o) == ({o} + (set oo <- o.owner, ooo <- oo.AMFO :: ooo));
+     forall oo <- o.owner ensures (oo.AMFO == argh(oo)) { argh_LEMMA0(oo); }
+     assert forall oo <- o.owner :: oo.AMFO == argh(oo);
+     assert argh(o) == ({o} + (set oo <- o.owner, ooo <- argh(oo) :: ooo));//ERR
+}
+
+lemma argh_LEMMA6(o : Object)
+  decreases o.AMFO
+   requires o.Ready()
+    ensures argh(o) == ({o} + (set oo <- o.owner, ooo <- argh(oo) :: ooo))//ERR
+{
+     argh_LEMMA4(o);
+     assert argh(o) == ({o} + (set oo <- o.owner, ooo <- oo.AMFO :: ooo));
+     forall oo <- o.owner ensures (oo.AMFO == argh(oo)) { argh_LEMMA0(oo); }
+     assert argh(o) == ({o} + (set oo <- o.owner, ooo <- argh(oo) :: ooo));//ERR
+}
+
+
+
 
 function amfoStrictlyInside(o : Object, pivot : Object) : Owner
   decreases o.AMFO
